Progress on porting P256 to the new libraries

code/p256/Hacl.Impl.P256.fst
@@ -1,39 +1,42 @@
 module Hacl.Impl.P256
 
-module ST = FStar.HyperStack.ST
-
-open FStar.HyperStack.All
-
-
 open FStar.Mul
 open FStar.HyperStack
-open FStar.Ghost
-open FStar.Buffer
-open FStar.Endianness
-open FStar.Int.Cast
+open FStar.HyperStack.ST
 
-open Hacl.Endianness
-open C.Loops
+open Lib.IntTypes
+open Lib.Sequence
+open Lib.ByteSequence
+open Lib.Buffer
+open Lib.Buffer.Lemmas
+
+module ST = FStar.HyperStack.ST
+module S = Lib.Sequence
+module BB = Lib.ByteBuffer
 
 (* Taken straight from the OpenSSL github code *)
 
+
+let to_shiftval x = size_to_uint32 (size x)
+
 (* Constants *)
-let nlimbs = 4
-let nlimbs' = 4ul
+let nlimbs : size_nat = 4
+let nlimbs' = u32 nlimbs
 
 (* Type aliases *)
-type u64 = UInt64.t
-type limb = UInt128.t
-type felem = b:buffer limb{length b = nlimbs}
-type longfelem = b:buffer limb{length b = 2 * nlimbs}
-type smallfelem = b:buffer u64{length b = nlimbs}
+type limb = uint128
+type felem = lbuffer limb nlimbs
+type longfelem = lbuffer limb (2 * nlimbs)
+type smallfelem = lbuffer uint64 nlimbs
+type bin32 = lbuffer uint8 32
+
 
 val create_felem:
   unit -> StackInline felem
     (requires (fun h -> True))
     (ensures (fun h0 _ h1 -> True))
 let create_felem () =
-  create (UInt128.uint64_to_uint128 0uL) 4ul
+  create (size 4) (u128 0)
 
 
 val create_longfelem:
@@ -41,135 +44,142 @@ val create_longfelem:
     (requires (fun h -> True))
     (ensures (fun h0 _ h1 -> True))
 let create_longfelem () =
-  create (UInt128.uint64_to_uint128 0uL) 8ul
+  create (size 8) (u128 0)
+
 
 val create_smallfelem:
   unit -> StackInline smallfelem
     (requires (fun h -> True))
     (ensures (fun h0 _ h1 -> True))
 let create_smallfelem () =
-  create 0uL 4ul
+  create (size 4) (u64 0)
 
-val kPrime: unit -> 
+
+val kPrime: unit ->
   StackInline smallfelem
     (requires (fun h -> True))
     (ensures (fun h0 b h1 -> True))
 let kPrime () =
-  let b = createL [0xffffffffffffffffuL; 0xffffffffuL; 0uL; 0xffffffff00000001uL] in
+  let b = createL [u64 0xffffffffffffffff; u64 0xffffffff; u64 0; u64 0xffffffff00000001] in
   b
 
+
 val bin32_to_felem:
-  output:felem -> input:buffer UInt8.t{length input = 32} ->
+  output:felem -> input:bin32 ->
   Stack unit
     (requires (fun h -> True))
     (ensures (fun h0 _ h1 -> True))
 let bin32_to_felem output input =
-  let in0 = Buffer.sub input 0ul  8ul in
-  let in1 = Buffer.sub input 8ul  8ul in
-  let in2 = Buffer.sub input 16ul 8ul in
-  let in3 = Buffer.sub input 24ul 8ul in
-  let o0 = load64_le in0 in
-  let o1 = load64_le in1 in
-  let o2 = load64_le in2 in
-  let o3 = load64_le in3 in
-  output.(0ul) <- UInt128.uint64_to_uint128 o0;
-  output.(1ul) <- UInt128.uint64_to_uint128 o1;
-  output.(2ul) <- UInt128.uint64_to_uint128 o2;
-  output.(3ul) <- UInt128.uint64_to_uint128 o3
+  let h0 = ST.get () in
+  alloc #h0 #uint64 #unit #limb (size 1) (u64 0) output
+  (fun h -> (fun _ sv -> True))
+  (fun w ->
+    let in0 = sub input (size 0) (size 8) in
+    let in1 = sub input (size 8)  (size 8) in
+    let in2 = sub input (size 16) (size 8) in
+    let in3 = sub input (size 24) (size 8) in
+    let w0 : uint64 = index #uint64 #1 w (size 0) in
+    BB.uints_from_bytes_le w (size 8) in0;
+    output.(size 0) <- to_u128 w0;
+    BB.uints_from_bytes_le w (size 8) in1;
+    output.(size 1) <- to_u128 w0;
+    BB.uints_from_bytes_le w (size 8) in2;
+    output.(size 2) <- to_u128 w0;
+    BB.uints_from_bytes_le w (size 8) in3;
+    output.(size 3) <- to_u128 w0
+  )
 
 
 val smallfelem_to_bin32:
-  output:buffer UInt8.t{length output = 32} -> input:smallfelem ->
+  output:bin32 -> input:smallfelem ->
   Stack unit
     (requires (fun h -> True))
     (ensures (fun h0 _ h1 -> True))
-let smallfelem_to_bin32 output input =
-  let o0 = Buffer.sub output 0ul  8ul in
-  let o1 = Buffer.sub output 8ul  8ul in
-  let o2 = Buffer.sub output 16ul 8ul in
-  let o3 = Buffer.sub output 24ul 8ul in
-  let in0 = input.(0ul) in
-  let in1 = input.(1ul) in
-  let in2 = input.(2ul) in
-  let in3 = input.(3ul) in
-  store64_le o0 in0;
-  store64_le o1 in1;
-  store64_le o2 in2;
-  store64_le o3 in3
+let smallfelem_to_bin32 output input = BB.uints_to_bytes_le output (size 8) input
+  (* let o0 : lbuffer uint8 8 = sub output (size 0) (size 8) in *)
+  (* let o1 : lbuffer uint8 8 = sub output (size 8) (size 8) in *)
+  (* let o2 : lbuffer uint8 8 = sub output (size 16) (size 8) in *)
+  (* let o3 : lbuffer uint8 8 = sub output (size 24) (size 8) in *)
+  (* let in0 : uint64 = input.(size 0) in *)
+  (* let in1 : uint64 = input.(size 1) in *)
+  (* let in2 : uint64 = input.(size 2) in *)
+  (* let in3 : uint64 = input.(size 3) in *)
+  (* BB.uint_to_bytes_le o0 in0; *)
+  (* BB.uint_to_bytes_le o1 in1; *)
+  (* BB.uint_to_bytes_le o2 in2; *)
+  (* BB.uint_to_bytes_le o3 in3 *)
 
 
 val flip_endian:
-  output:buffer UInt8.t{length output = 32} -> input:buffer UInt8.t{length input = 32} -> len:UInt32.t ->
+  output:bin32 -> input:bin32 -> len:size_t ->
   Stack unit
     (requires (fun h -> True))
     (ensures (fun h0 _ h1 -> True))
 let flip_endian output input len =
-  let inv (h1:mem) (i:nat) = True in
-  let f (i:UInt32.t) : Stack unit
-    (requires (fun h -> True))
-    (ensures (fun h0 _ h1 -> True))
-    = let inputim1 = input.(FStar.UInt32.(len -^ 1ul -^ i)) in
-      output.(i) <- inputim1 in
-  for 0ul len inv f
+  (**) let h0 = ST.get () in
+  loop_nospec #h0 len output
+  (fun i ->
+    let idx = len -. (size 1) -. i in
+    let inputim1 = input.(idx) in
+    output.(i) <- inputim1)
+
 
 (* Field operations *)
-
 val smallfelem_one: out:smallfelem ->
   Stack unit
     (requires (fun h -> True))
     (ensures (fun h0 _ h1 -> True))
 let smallfelem_one out =
-  out.(0ul) <- 1uL;
-  out.(1ul) <- 0uL;
-  out.(2ul) <- 0uL;
-  out.(3ul) <- 0uL
+  out.(size 0) <- u64 1;
+  out.(size 1) <- u64 0;
+  out.(size 2) <- u64 0;
+  out.(size 3) <- u64 0
 
 val smallfelem_assign: out:smallfelem -> input:smallfelem ->
   Stack unit
     (requires (fun h -> True))
     (ensures (fun h0 _ h1 -> True))
 let smallfelem_assign out input =
-  let in0 = input.(0ul) in
-  let in1 = input.(1ul) in
-  let in2 = input.(2ul) in
-  let in3 = input.(3ul) in
-  out.(0ul) <- in0;
-  out.(1ul) <- in1;
-  out.(2ul) <- in2;
-  out.(3ul) <- in3
+  let in0 = input.(size 0) in
+  let in1 = input.(size 1) in
+  let in2 = input.(size 2) in
+  let in3 = input.(size 3) in
+  out.(size 0) <- in0;
+  out.(size 1) <- in1;
+  out.(size 2) <- in2;
+  out.(size 3) <- in3
 
 val felem_assign: out:felem -> input:felem ->
   Stack unit
     (requires (fun h -> True))
     (ensures (fun h0 _ h1 -> True))
 let felem_assign out input =
-  let in0 = input.(0ul) in
-  let in1 = input.(1ul) in
-  let in2 = input.(2ul) in
-  let in3 = input.(3ul) in
-  out.(0ul) <- in0;
-  out.(1ul) <- in1;
-  out.(2ul) <- in2;
-  out.(3ul) <- in3
+  let in0 = input.(size 0) in
+  let in1 = input.(size 1) in
+  let in2 = input.(size 2) in
+  let in3 = input.(size 3) in
+  out.(size 0) <- in0;
+  out.(size 1) <- in1;
+  out.(size 2) <- in2;
+  out.(size 3) <- in3
 
 val felem_sum: out:felem -> input:felem ->
   Stack unit
     (requires (fun h -> True))
     (ensures (fun h0 _ h1 -> True))
 let felem_sum out input =
-  let in0 = input.(0ul) in
-  let in1 = input.(1ul) in
-  let in2 = input.(2ul) in
-  let in3 = input.(3ul) in
-  let o0 = out.(0ul) in
-  let o1 = out.(1ul) in
-  let o2 = out.(2ul) in
-  let o3 = out.(3ul) in
-  let open FStar.UInt128 in
-  out.(0ul) <- o0 +^ in0;
-  out.(1ul) <- o1 +^ in1;
-  out.(2ul) <- o2 +^ in2;
-  out.(3ul) <- o3 +^ in3
+  let in0 = input.(size 0) in
+  let in1 = input.(size 1) in
+  let in2 = input.(size 2) in
+  let in3 = input.(size 3) in
+  let o0 = out.(size 0) in
+  let o1 = out.(size 1) in
+  let o2 = out.(size 2) in
+  let o3 = out.(size 3) in
+  out.(size 0) <- o0 +. in0;
+  out.(size 1) <- o1 +. in1;
+  out.(size 2) <- o2 +. in2;
+  out.(size 3) <- o3 +. in3
 
 
 val felem_small_sum: out:felem -> input:smallfelem ->
@@ -177,113 +187,108 @@ val felem_small_sum: out:felem -> input:smallfelem ->
     (requires (fun h -> True))
     (ensures (fun h0 _ h1 -> True))
 let felem_small_sum out input =
-  let in0 = input.(0ul) in
-  let in1 = input.(1ul) in
-  let in2 = input.(2ul) in
-  let in3 = input.(3ul) in
-  let o0 = out.(0ul) in
-  let o1 = out.(1ul) in
-  let o2 = out.(2ul) in
-  let o3 = out.(3ul) in
+  let in0 = input.(size 0) in
+  let in1 = input.(size 1) in
+  let in2 = input.(size 2) in
+  let in3 = input.(size 3) in
+  let o0 = out.(size 0) in
+  let o1 = out.(size 1) in
+  let o2 = out.(size 2) in
+  let o3 = out.(size 3) in
   let open FStar.UInt128 in
-  out.(0ul) <- o0 +^ uint64_to_uint128 in0;
-  out.(1ul) <- o1 +^ uint64_to_uint128 in1;
-  out.(2ul) <- o2 +^ uint64_to_uint128 in2;
-  out.(3ul) <- o3 +^ uint64_to_uint128 in3
+  out.(size 0) <- o0 +. to_u128 in0;
+  out.(size 1) <- o1 +. to_u128 in1;
+  out.(size 2) <- o2 +. to_u128 in2;
+  out.(size 3) <- o3 +. to_u128 in3
 
 
 // TODO: check that the downcast to u64 is indeed correct, otherwise this
 // requires a special implementation of the multiplication
-val felem_scalar: out:felem -> scalar:u32 ->
+val felem_scalar: out:felem -> scalar:shiftval U128 ->
   Stack unit
     (requires (fun h -> True))
     (ensures (fun h0 _ h1 -> True))
 let felem_scalar out scalar =
-  let open FStar.UInt128 in
-  let o0 = out.(0ul) in
-  let o1 = out.(1ul) in
-  let o2 = out.(2ul) in
-  let o3 = out.(3ul) in
+  let o0 = out.(size 0) in
+  let o1 = out.(size 1) in
+  let o2 = out.(size 2) in
+  let o3 = out.(size 3) in
   // let o0 = uint128_to_uint64 o0 in
   // let o1 = uint128_to_uint64 o1 in
   // let o2 = uint128_to_uint64 o2 in
   // let o3 = uint128_to_uint64 o3 in
-  let scalar = scalar in
-  out.(0ul) <- shift_left o0 scalar;
-  out.(1ul) <- shift_left o1 scalar;
-  out.(2ul) <- shift_left o2 scalar;
-  out.(3ul) <- shift_left o3 scalar
+  (* let scalar = scalar in *)
+  out.(size 0) <- shift_left o0 scalar;
+  out.(size 1) <- shift_left o1 scalar;
+  out.(size 2) <- shift_left o2 scalar;
+  out.(size 3) <- shift_left o3 scalar
 
 
 // TODO: check that the downcast to u64 is indeed correct, otherwise this
 // requires a special implementation of the multiplication
-val longfelem_scalar: out:longfelem -> scalar:u32 ->
+val longfelem_scalar: out:longfelem -> scalar:shiftval U128 ->
   Stack unit
     (requires (fun h -> True))
     (ensures (fun h0 _ h1 -> True))
 let longfelem_scalar out scalar =
-  let open FStar.UInt128 in
-  let o0 = out.(0ul) in
-  let o1 = out.(1ul) in
-  let o2 = out.(2ul) in
-  let o3 = out.(3ul) in
-  let o4 = out.(4ul) in
-  let o5 = out.(5ul) in
-  let o6 = out.(6ul) in
-  let o7 = out.(7ul) in
-  let scalar = scalar in
-  out.(0ul) <- shift_left o0 scalar;
-  out.(1ul) <- shift_left o1 scalar;
-  out.(2ul) <- shift_left o2 scalar;
-  out.(3ul) <- shift_left o3 scalar;
-  out.(4ul) <- shift_left o4 scalar;
-  out.(5ul) <- shift_left o5 scalar;
-  out.(6ul) <- shift_left o6 scalar;
-  out.(7ul) <- shift_left o7 scalar
-  // out.(0ul) <- mul_wide o0 scalar;
-  // out.(1ul) <- mul_wide o1 scalar;
-  // out.(2ul) <- mul_wide o2 scalar;
-  // out.(3ul) <- mul_wide o3 scalar;
-  // out.(4ul) <- mul_wide o4 scalar;
-  // out.(5ul) <- mul_wide o5 scalar;
-  // out.(6ul) <- mul_wide o6 scalar;
-  // out.(7ul) <- mul_wide o7 scalar
+  let o0 = out.(size 0) in
+  let o1 = out.(size 1) in
+  let o2 = out.(size 2) in
+  let o3 = out.(size 3) in
+  let o4 = out.(size 4) in
+  let o5 = out.(size 5) in
+  let o6 = out.(size 6) in
+  let o7 = out.(size 7) in
+  out.(size 0) <- shift_left o0 scalar;
+  out.(size 1) <- shift_left o1 scalar;
+  out.(size 2) <- shift_left o2 scalar;
+  out.(size 3) <- shift_left o3 scalar;
+  out.(size 4) <- shift_left o4 scalar;
+  out.(size 5) <- shift_left o5 scalar;
+  out.(size 6) <- shift_left o6 scalar;
+  out.(size 7) <- shift_left o7 scalar
+  // out.(0) <- mul_wide o0 scalar;
+  // out.(1) <- mul_wide o1 scalar;
+  // out.(2) <- mul_wide o2 scalar;
+  // out.(3) <- mul_wide o3 scalar;
+  // out.(4) <- mul_wide o4 scalar;
+  // out.(5) <- mul_wide o5 scalar;
+  // out.(6) <- mul_wide o6 scalar;
+  // out.(7) <- mul_wide o7 scalar
 
 inline_for_extraction
-val load128: high:UInt64.t -> low:UInt64.t -> Tot (z:UInt128.t{UInt128.v z = pow2 64 * UInt64.v high
-  + UInt64.v low})
+val load128: high:uint64 -> low:uint64 -> Tot (z:uint128{uint_v z = pow2 64 * (uint_v high) + (uint_v low)})
 let load128 h l =
-  let open FStar.UInt128 in
-  let hs = uint64_to_uint128 h <<^ 64ul in
-  let ls = uint64_to_uint128 l in
-  Math.Lemmas.modulo_lemma (UInt64.v h * pow2 64) (pow2 128);
-  UInt.logor_disjoint #128 (v hs) (v ls) 64;
-  hs |^ ls
+  let hs = to_u128 h <<. (size_to_uint32 (size 64)) in
+  let ls = to_u128 l in
+  (* Math.Lemmas.modulo_lemma (UInt64.v h * pow2 64) (pow2 128); *)
+  (* UInt.logor_disjoint #128 (v hs) (v ls) 64; *)
+  hs |. ls
 
 
 (* Put in uint128 form*)
-let two105m41m9 = load128 0x1ffffffffffuL 0xfffffdfffffffe00uL
-let two105      = load128 0x20000000000uL 0x0uL
-let two105m41p9 = load128 0x1ffffffffffuL 0xfffffe0000000200uL
+let two105m41m9 = load128 (u64 0x1ffffffffff) (u64 0xfffffdfffffffe00)
+let two105      = load128 (u64 0x20000000000) (u64 0)
+let two105m41p9 = load128 (u64 0x1ffffffffff) (u64 0xfffffe0000000200)
 
-let two107m43m11 = load128 0x7ffffffffffuL 0xfffff7fffffff800uL
-let two107       = load128 0x80000000000uL 0x0uL
-let two107m43p11 = load128 0x7ffffffffffuL 0xfffff80000000800uL
+let two107m43m11 = load128 (u64 0x7ffffffffff) (u64 0xfffff7fffffff800)
+let two107       = load128 (u64 0x80000000000) (u64 0)
+let two107m43p11 = load128 (u64 0x7ffffffffff) (u64 0xfffff80000000800)
 
-let two64m0     = UInt128.uint64_to_uint128 0xffffffffffffffffuL
-let two110p32m0 = load128 0x400000000000uL 0x00000000ffffffffuL
-let two64m46    = UInt128.uint64_to_uint128 0xffffc00000000000uL
-let two64m32    = UInt128.uint64_to_uint128 0xffffffff00000000uL
+let two64m0     = to_u128 (u64 0xffffffffffffffff)
+let two110p32m0 = load128 (u64 0x400000000000) (u64 0x00000000ffffffff)
+let two64m46    = to_u128 (u64 0xffffc00000000000)
+let two64m32    = to_u128 (u64 0xffffffff00000000)
 
-let two70m8p6     = load128 0x3fuL 0xffffffffffffff40uL
-let two70p40      = load128 0x40uL 0x0000010000000000uL
-let two70         = load128 0x40uL 0x0000000000000000uL
-let two70m40m38p6 = load128 0x3fuL 0xfffffec000000040uL
-let two70m6       = load128 0x3fuL 0xffffffffffffffc0uL
+let two70m8p6     = load128 (u64 0x3f) (u64 0xffffffffffffff40)
+let two70p40      = load128 (u64 0x40) (u64 0x0000010000000000)
+let two70         = load128 (u64 0x40) (u64 0x0000000000000000)
+let two70m40m38p6 = load128 (u64 0x3f) (u64 0xfffffec000000040)
+let two70m6       = load128 (u64 0x3f) (u64 0xffffffffffffffc0)
 
-let two100m36m4 = load128 0xfffffffffuL 0xffffffeffffffff0uL
-let two100      = load128 0x1000000000uL 0x0uL
-let two100m36p4 = load128 0xfffffffffuL 0xfffffff000000010uL
+let two100m36m4 = load128 (u64 0xfffffffff) (u64 0xffffffeffffffff0)
+let two100      = load128 (u64 0x1000000000) (u64 0x0)
+let two100m36p4 = load128 (u64 0xfffffffff) (u64 0xfffffff000000010)
 
 
 val zero105: unit -> StackInline felem
@@ -311,22 +316,19 @@ val smallfelem_neg: out:felem -> small:smallfelem -> Stack unit
   (requires (fun h -> True))
   (ensures (fun h0 _ h1 -> True))
 let smallfelem_neg out small =
-  push_frame();
   let zero105 = zero105 () in
-  let open FStar.UInt128 in
-  let small0 = small.(0ul) in
-  let small1 = small.(1ul) in
-  let small2 = small.(2ul) in
-  let small3 = small.(3ul) in
-  let zero0  = zero105.(0ul) in
-  let zero1  = zero105.(1ul) in
-  let zero2  = zero105.(2ul) in
-  let zero3  = zero105.(3ul) in
-  out.(0ul) <- zero0 -^ uint64_to_uint128 small0;
-  out.(1ul) <- zero1 -^ uint64_to_uint128 small1;
-  out.(2ul) <- zero2 -^ uint64_to_uint128 small2;
-  out.(3ul) <- zero3 -^ uint64_to_uint128 small3;
-  pop_frame()
+  let small0 = small.(size 0) in
+  let small1 = small.(size 1) in
+  let small2 = small.(size 2) in
+  let small3 = small.(size 3) in
+  let zero0  = zero105.(size 0) in
+  let zero1  = zero105.(size 1) in
+  let zero2  = zero105.(size 2) in
+  let zero3  = zero105.(size 3) in
+  out.(size 0) <- zero0 -. (to_u128 small0);
+  out.(size 1) <- zero1 -. (to_u128 small1);
+  out.(size 2) <- zero2 -. (to_u128 small2);
+  out.(size 3) <- zero3 -. (to_u128 small3)
 
 val felem_diff:
   out:felem -> input:felem -> Stack unit
@@ -336,26 +338,26 @@ let felem_diff out input =
   push_frame();
   let zero105 = zero105 () in
   let open FStar.UInt128 in
-  let input0 = input.(0ul) in
-  let input1 = input.(1ul) in
-  let input2 = input.(2ul) in
-  let input3 = input.(3ul) in
-  let out0 = out.(0ul) in
-  let out1 = out.(1ul) in
-  let out2 = out.(2ul) in
-  let out3 = out.(3ul) in
-  let zero0  = zero105.(0ul) in
-  let zero1  = zero105.(1ul) in
-  let zero2  = zero105.(2ul) in
-  let zero3  = zero105.(3ul) in
-  let out0 = zero0 +^ out0 in
-  let out1 = zero1 +^ out1 in
-  let out2 = zero2 +^ out2 in
-  let out3 = zero3 +^ out3 in
-  out.(0ul) <- out0 -^ input0;
-  out.(1ul) <- out1 -^ input1;
-  out.(2ul) <- out2 -^ input2;
-  out.(3ul) <- out3 -^ input3;
+  let input0 = input.(size 0) in
+  let input1 = input.(size 1) in
+  let input2 = input.(size 2) in
+  let input3 = input.(size 3) in
+  let out0 = out.(size 0) in
+  let out1 = out.(size 1) in
+  let out2 = out.(size 2) in
+  let out3 = out.(size 3) in
+  let zero0  = zero105.(size 0) in
+  let zero1  = zero105.(size 1) in
+  let zero2  = zero105.(size 2) in
+  let zero3  = zero105.(size 3) in
+  let out0 = zero0 +. out0 in
+  let out1 = zero1 +. out1 in
+  let out2 = zero2 +. out2 in
+  let out3 = zero3 +. out3 in
+  out.(size 0) <- out0 -. input0;
+  out.(size 1) <- out1 -. input1;
+  out.(size 2) <- out2 -. input2;
+  out.(size 3) <- out3 -. input3;
   pop_frame()
 
 
@@ -366,27 +368,26 @@ val felem_diff_zero107:
 let felem_diff_zero107 out input =
   push_frame();
   let zero107 = zero107 () in
-  let open FStar.UInt128 in
-  let input0 = input.(0ul) in
-  let input1 = input.(1ul) in
-  let input2 = input.(2ul) in
-  let input3 = input.(3ul) in
-  let out0 = out.(0ul) in
-  let out1 = out.(1ul) in
-  let out2 = out.(2ul) in
-  let out3 = out.(3ul) in
-  let zero0  = zero107.(0ul) in
-  let zero1  = zero107.(1ul) in
-  let zero2  = zero107.(2ul) in
-  let zero3  = zero107.(3ul) in
-  let out0 = zero0 +^ out0 in
-  let out1 = zero1 +^ out1 in
-  let out2 = zero2 +^ out2 in
-  let out3 = zero3 +^ out3 in
-  out.(0ul) <- out0 -^ input0;
-  out.(1ul) <- out1 -^ input1;
-  out.(2ul) <- out2 -^ input2;
-  out.(3ul) <- out3 -^ input3;
+  let input0 = input.(size 0) in
+  let input1 = input.(size 1) in
+  let input2 = input.(size 2) in
+  let input3 = input.(size 3) in
+  let out0 = out.(size 0) in
+  let out1 = out.(size 1) in
+  let out2 = out.(size 2) in
+  let out3 = out.(size 3) in
+  let zero0  = zero107.(size 0) in
+  let zero1  = zero107.(size 1) in
+  let zero2  = zero107.(size 2) in
+  let zero3  = zero107.(size 3) in
+  let out0 = zero0 +. out0 in
+  let out1 = zero1 +. out1 in
+  let out2 = zero2 +. out2 in
+  let out3 = zero3 +. out3 in
+  out.(size 0) <- out0 -. input0;
+  out.(size 1) <- out1 -. input1;
+  out.(size 2) <- out2 -. input2;
+  out.(size 3) <- out3 -. input3;
   pop_frame()
 
 
@@ -396,39 +397,38 @@ val longfelem_diff:
     (ensures (fun h0 _ h1 -> True))
 let longfelem_diff out input =
   push_frame();
-  let open FStar.UInt128 in
-  let input0 = input.(0ul) in
-  let input1 = input.(1ul) in
-  let input2 = input.(2ul) in
-  let input3 = input.(3ul) in
-  let input4 = input.(4ul) in
-  let input5 = input.(5ul) in
-  let input6 = input.(6ul) in
-  let input7 = input.(7ul) in
-  let out0 = out.(0ul) in
-  let out1 = out.(1ul) in
-  let out2 = out.(2ul) in
-  let out3 = out.(3ul) in
-  let out4 = out.(4ul) in
-  let out5 = out.(5ul) in
-  let out6 = out.(6ul) in
-  let out7 = out.(7ul) in
-  let out0 =  two70m8p6 +^ out0 in
-  let out1 = two70p40 +^ out1 in
-  let out2 = two70 +^ out2 in
-  let out3 = two70m40m38p6 +^ out3 in
-  let out4 = two70m6 +^ out4 in
-  let out5 = two70m6 +^ out5 in
-  let out6 = two70m6 +^ out6 in
-  let out7 = two70m6 +^ out7 in
-  out.(0ul) <- out0 -^ input0;
-  out.(1ul) <- out1 -^ input1;
-  out.(2ul) <- out2 -^ input2;
-  out.(3ul) <- out3 -^ input3;
-  out.(4ul) <- out4 -^ input4;
-  out.(5ul) <- out5 -^ input5;
-  out.(6ul) <- out6 -^ input6;
-  out.(7ul) <- out7 -^ input7;
+  let input0 = input.(size 0) in
+  let input1 = input.(size 1) in
+  let input2 = input.(size 2) in
+  let input3 = input.(size 3) in
+  let input4 = input.(size 4) in
+  let input5 = input.(size 5) in
+  let input6 = input.(size 6) in
+  let input7 = input.(size 7) in
+  let out0 = out.(size 0) in
+  let out1 = out.(size 1) in
+  let out2 = out.(size 2) in
+  let out3 = out.(size 3) in
+  let out4 = out.(size 4) in
+  let out5 = out.(size 5) in
+  let out6 = out.(size 6) in
+  let out7 = out.(size 7) in
+  let out0 =  two70m8p6 +. out0 in
+  let out1 = two70p40 +. out1 in
+  let out2 = two70 +. out2 in
+  let out3 = two70m40m38p6 +. out3 in
+  let out4 = two70m6 +. out4 in
+  let out5 = two70m6 +. out5 in
+  let out6 = two70m6 +. out6 in
+  let out7 = two70m6 +. out7 in
+  out.(size 0) <- out0 -. input0;
+  out.(size 1) <- out1 -. input1;
+  out.(size 2) <- out2 -. input2;
+  out.(size 3) <- out3 -. input3;
+  out.(size 4) <- out4 -. input4;
+  out.(size 5) <- out5 -. input5;
+  out.(size 6) <- out6 -. input6;
+  out.(size 7) <- out7 -. input7;
   pop_frame()
 
 
@@ -439,81 +439,82 @@ val felem_shrink:
     (ensures (fun h0 _ h1 -> True))
 let felem_shrink out input =
   push_frame();
-  let tmp = create (FStar.UInt128.uint64_to_uint128 0uL) 4ul in
+  let tmp = create #uint128 #4 (size 4) (u128 0) in
   let zero110 = zero110 () in
   let kPrime  = kPrime () in
-  let kPrime3Test = 0x7fffffff00000001uL in
-  let input0 = input.(0ul) in
-  let input1 = input.(1ul) in
-  let input2 = input.(2ul) in
-  let input3 = input.(3ul) in
-  let zero0  = zero110.(0ul) in
-  let zero1  = zero110.(1ul) in
-  let zero2  = zero110.(2ul) in
-  let zero3  = zero110.(3ul) in
-  let kPrime0 = kPrime.(0ul) in
-  let kPrime1 = kPrime.(1ul) in
-  let kPrime2 = kPrime.(2ul) in
-  let kPrime3 = kPrime.(3ul) in
-  let open FStar.UInt128 in
+  let kPrime3Test = (u64 0x7fffffff00000001) in
+  let input0 = input.(size 0) in
+  let input1 = input.(size 1) in
+  let input2 = input.(size 2) in
+  let input3 = input.(size 3) in
+  let zero0  = zero110.(size 0) in
+  let zero1  = zero110.(size 1) in
+  let zero2  = zero110.(size 2) in
+  let zero3  = zero110.(size 3) in
+  let kPrime0 = kPrime.(size 0) in
+  let kPrime1 = kPrime.(size 1) in
+  let kPrime2 = kPrime.(size 2) in
+  let kPrime3 = kPrime.(size 3) in
   // TODO: replace with a primitive to call the high word only
-  let tmp3 = zero3 +^ input3 +^ (input2 >>^ 64ul) in
-  // tmp.(3ul) <- zero3 +^ input3 +^ (input2 >>^ 64ul);
-  let tmp2 = zero2 +^ (uint64_to_uint128 (uint128_to_uint64 input2)) in
-  // tmp.(2ul) <- zero2 +^ (uint64_to_uint128 (uint128_to_uint64 input2));
-  let tmp0 = zero0 +^ input0 in
-  // tmp.(0ul) <- zero0 +^ input0;
-  let tmp1 = zero1 +^ input1 in
-  // tmp.(1ul) <- zero1 +^ input1;
+  let tmp3 = zero3 +. input3 +. (input2 >>. (size_to_uint32 (size 64))) in
+  // tmp.(3ul) <- zero3 +. input3 +. (input2 >>^ 64ul);
+  let tmp2 = zero2 +. (to_u128 (to_u64 input2)) in
+// BB.  let tmp2 = zero2 +. (uint64_to_uint128 (uint128_to_uint64 input2)) in
+  // tmp.(2ul) <- zero2 +. (uint64_to_uint128 (uint128_to_uint64 input2));
+  let tmp0 = zero0 +. input0 in
+  // tmp.(0ul) <- zero0 +. input0;
+  let tmp1 = zero1 +. input1 in
+  // tmp.(1ul) <- zero1 +. input1;
 
   // let tmp2 = tmp.(2ul) in
   // let tmp3 = tmp.(3ul) in
-  let a = tmp3 >>^ 64ul in
-  let tmp3 = uint64_to_uint128 (uint128_to_uint64 tmp3) in
-  let tmp3 = tmp3 -^ a in
-  let tmp3 = tmp3 +^ (a <<^ 32ul) in
+  let a = tmp3 >>. (size_to_uint32 (size 64)) in
+  let tmp3 = to_u128 (to_u64 tmp3) in
+// BB.  (* let tmp3 = uint64_to_uint128 (uint128_to_uint64 tmp3) in *)
+  let tmp3 = tmp3 -. a in
+  let tmp3 = tmp3 +. (a <<. (size_to_uint32 (size 32))) in
 
   let b = a in
-  let a = tmp3 >>^ 64ul in
-  let b = b +^ a in
-  let tmp3 = uint64_to_uint128 (uint128_to_uint64 tmp3) in
-  let tmp3 = tmp3 -^ a in
-  let tmp3 = tmp3 +^ (a <<^ 32ul) in
+  let a = tmp3 >>. (size_to_uint32 (size 64)) in
+  let b = b +. a in
+  let tmp3 = to_u128 (to_u64 tmp3) in
+  let tmp3 = tmp3 -. a in
+  let tmp3 = tmp3 +. (a <<. (size_to_uint32 (size 32))) in
 
   // let tmp0 = tmp.(0ul) in
-  let tmp0 = tmp0 +^ b in
+  let tmp0 = tmp0 +. b in
   // let tmp1 = tmp.(1ul) in
-  let tmp1 = tmp1 -^ (b <<^ 32ul) in
+  let tmp1 = tmp1 -. (b <<. (size_to_uint32 (size 32))) in
 
   // TODO: better implementation
   // let high = tmp3 >>^ 64ul in
-  let high = uint128_to_uint64 (gte_mask tmp3 (load128 0x1uL 0x0uL)) in
+  let high = to_u64 (gte_mask tmp3 (load128 (u64 0x1) (u64 0x0))) in
 
   // TODO: better implementation
-  let low = uint128_to_uint64 tmp3 in
-  let mask = UInt64.gte_mask low 0x8000000000000000uL in
+  let low = to_u64 tmp3 in
+  let mask = gte_mask low (u64 0x8000000000000000) in
 
-  let low = FStar.UInt64.(low &^ 0x7fffffffffffffffuL) in
-  let low = UInt64.gte_mask kPrime3Test low in
-  let low = UInt64.lognot low in
+  let low = low &. (u64 0x7fffffffffffffff) in
+  let low = gte_mask kPrime3Test low in
+  let low = lognot low in
 
-  let mask = FStar.UInt64.((mask &^ low) |^ high) in
+  let mask = ((mask &. low) |. high) in
 
-  let tmp0 = tmp0 -^ uint64_to_uint128 FStar.UInt64.(mask &^ kPrime0) in
-  let tmp1 = tmp1 -^ uint64_to_uint128 FStar.UInt64.(mask &^ kPrime1) in
-  let tmp3 = tmp3 -^ uint64_to_uint128 FStar.UInt64.(mask &^ kPrime3) in
+  let tmp0 = tmp0 -. to_u128 (mask &. kPrime0) in
+  let tmp1 = tmp1 -. to_u128 (mask &. kPrime1) in
+  let tmp3 = tmp3 -. to_u128 (mask &. kPrime3) in
 
-  let tmp1 = tmp1 +^ (tmp0 >>^ 64ul) in
-  let tmp0 = uint128_to_uint64 tmp0 in
-  let tmp2 = tmp2 +^ (tmp1 >>^ 64ul) in
-  let tmp1 = uint128_to_uint64 tmp1 in
-  let tmp3 = tmp3 +^ (tmp2 >>^ 64ul) in
-  let tmp2 = uint128_to_uint64 tmp2 in
+  let tmp1 = tmp1 +. (tmp0 >>. (size_to_uint32 (size 64))) in
+  let tmp0 = to_u64 tmp0 in
+  let tmp2 = tmp2 +. (tmp1 >>. (to_shiftval 64)) in
+  let tmp1 = to_u64 tmp1 in
+  let tmp3 = tmp3 +. (tmp2 >>. (to_shiftval 64)) in
+  let tmp2 = to_u64 tmp2 in
 
-  out.(0ul) <- tmp0;
-  out.(1ul) <- tmp1;
-  out.(2ul) <- tmp2;
-  out.(3ul) <- uint128_to_uint64 tmp3;
+  out.(size 0) <- tmp0;
+  out.(size 1) <- tmp1;
+  out.(size 2) <- tmp2;
+  out.(size 3) <- to_u64 tmp3;
   pop_frame ()
 
 
@@ -522,101 +523,99 @@ val smallfelem_expand:
     (requires (fun h -> True))
     (ensures (fun h0 _ h1 -> True))
 let smallfelem_expand out input =
-  let input0 = input.(0ul) in
-  let input1 = input.(1ul) in
-  let input2 = input.(2ul) in
-  let input3 = input.(3ul) in
-  let open FStar.UInt128 in
-  out.(0ul) <- uint64_to_uint128 input0;
-  out.(1ul) <- uint64_to_uint128 input1;
-  out.(2ul) <- uint64_to_uint128 input2;
-  out.(3ul) <- uint64_to_uint128 input3
+  let input0 = input.(size 0) in
+  let input1 = input.(size 1) in
+  let input2 = input.(size 2) in
+  let input3 = input.(size 3) in
+  out.(size 0) <- to_u128 input0;
+  out.(size 1) <- to_u128 input1;
+  out.(size 2) <- to_u128 input2;
+  out.(size 3) <- to_u128 input3
 
 val smallfelem_square:
   out:longfelem -> small:smallfelem -> Stack unit
     (requires (fun h -> True))
     (ensures (fun h0 _ h1 -> True))
 let smallfelem_square out small =
-  let open FStar.UInt128 in
-  let small0 = small.(0ul) in
-  let small1 = small.(1ul) in
-  let small2 = small.(2ul) in
-  let small3 = small.(3ul) in
+  let small0 = small.(size 0) in
+  let small1 = small.(size 1) in
+  let small2 = small.(size 2) in
+  let small3 = small.(size 3) in
 
   let a = mul_wide small0 small0 in
-  let low = uint64_to_uint128 (uint128_to_uint64 a) in
-  let high = a >>^ 64ul in
+  let low = to_u128 (to_u64 a) in
+  let high = a >>. to_shiftval 64 in
   let out0 = low in
   let out1 = high in
 
   let a = mul_wide small0 small1 in
-  let low = uint64_to_uint128 (uint128_to_uint64 a) in
-  let high = a >>^ 64ul in
-  let out1 = out1 +^ low in
-  let out1 = out1 +^ low in
+  let low = to_u128 (to_u64 a) in
+  let high = a >>. (to_shiftval 64) in
+  let out1 = out1 +. low in
+  let out1 = out1 +. low in
   let out2 = high in
 
   let a = mul_wide small0 small2 in
-  let low = uint64_to_uint128 (uint128_to_uint64 a) in
-  let high = a >>^ 64ul in
-  let out2 = out2 +^ low in
-  let out2 = out2 <<^ 1ul in
+  let low = to_u128 (to_u64 a) in
+  let high = a >>. to_shiftval 64 in
+  let out2 = out2 +. low in
+  let out2 = out2 <<. to_shiftval 1 in
   let out3 = high in
 
   let a = mul_wide small0 small3 in
-  let low = uint64_to_uint128 (uint128_to_uint64 a) in
-  let high = a >>^ 64ul in
-  let out3 = out3 +^ low in
+  let low = to_u128 (to_u64 a) in
+  let high = a >>. to_shiftval 64 in
+  let out3 = out3 +. low in
   let out4 = high in
 
   let a = mul_wide small1 small2 in
-  let low = uint64_to_uint128 (uint128_to_uint64 a) in
-  let high = a >>^ 64ul in
-  let out3 = out3 +^ low in
-  let out3 = out3 <<^ 1ul in
-  let out4 = out4 +^ high in
+  let low = to_u128 (to_u64 a) in
+  let high = a >>. to_shiftval 64 in
+  let out3 = out3 +. low in
+  let out3 = out3 <<. to_shiftval 1 in
+  let out4 = out4 +. high in
 
   let a = mul_wide small1 small1 in
-  let low = uint64_to_uint128 (uint128_to_uint64 a) in
-  let high = a >>^ 64ul in
-  let out2 = out2 +^ low in
-  let out3 = out3 +^ high in
+  let low = to_u128 (to_u64 a) in
+  let high = a >>. to_shiftval 64 in
+  let out2 = out2 +. low in
+  let out3 = out3 +. high in
 
   let a = mul_wide small1 small3 in
-  let low = uint64_to_uint128 (uint128_to_uint64 a) in
-  let high = a >>^ 64ul in
-  let out4 = out4 +^ low in
-  let out4 = out4 <<^ 1ul in
+  let low = to_u128 (to_u64 a) in
+  let high = a >>. to_shiftval 64 in
+  let out4 = out4 +. low in
+  let out4 = out4 <<. to_shiftval 1 in
   let out5 = high in
 
   let a = mul_wide small2 small3 in
-  let low = uint64_to_uint128 (uint128_to_uint64 a) in
-  let high = a >>^ 64ul in
-  let out5 = out5 +^ low in
-  let out5 = out5 <<^ 1ul in
+  let low = to_u128 (to_u64 a) in
+  let high = a >>. to_shiftval 64 in
+  let out5 = out5 +. low in
+  let out5 = out5 <<. to_shiftval 1 in
   let out6 = high in
-  let out6 = out6 +^ high in
+  let out6 = out6 +. high in
 
   let a = mul_wide small2 small2 in
-  let low = uint64_to_uint128 (uint128_to_uint64 a) in
-  let high = a >>^ 64ul in
-  let out4 = out4 +^ low in
-  let out5 = out5 +^ high in
+  let low = to_u128 (to_u64 a) in
+  let high = a >>. to_shiftval 64 in
+  let out4 = out4 +. low in
+  let out5 = out5 +. high in
 
   let a = mul_wide small3 small3 in
-  let low = uint64_to_uint128 (uint128_to_uint64 a) in
-  let high = a >>^ 64ul in
-  let out6 = out6 +^ low in
+  let low = to_u128 (to_u64 a) in
+  let high = a >>. to_shiftval 64 in
+  let out6 = out6 +. low in
   let out7 = high in
 
-  out.(0ul) <- out0;
-  out.(1ul) <- out1;
-  out.(2ul) <- out2;
-  out.(3ul) <- out3;
-  out.(4ul) <- out4;
-  out.(5ul) <- out5;
-  out.(6ul) <- out6;
-  out.(7ul) <- out7
+  out.(size 0) <- out0;
+  out.(size 1) <- out1;
+  out.(size 2) <- out2;
+  out.(size 3) <- out3;
+  out.(size 4) <- out4;
+  out.(size 5) <- out5;
+  out.(size 6) <- out6;
+  out.(size 7) <- out7
 
 
 val felem_square:
@@ -625,7 +624,7 @@ val felem_square:
     (ensures (fun h0 _ h1 -> True))
 let felem_square out input =
   push_frame();
-  let small = create 0uL 4ul in
+  let small = create (size 4) (u64 0) in
   felem_shrink small input;
   smallfelem_square out small;
   pop_frame()
@@ -636,120 +635,119 @@ val smallfelem_mul:
     (requires (fun h -> True))
     (ensures (fun h0 _ h1 -> True))
 let smallfelem_mul out small1 small2 =
-  let small10 = small1.(0ul) in
-  let small11 = small1.(1ul) in
-  let small12 = small1.(2ul) in
-  let small13 = small1.(3ul) in
-  let small20 = small2.(0ul) in
-  let small21 = small2.(1ul) in
-  let small22 = small2.(2ul) in
-  let small23 = small2.(3ul) in
+  let small10 = small1.(size 0) in
+  let small11 = small1.(size 1) in
+  let small12 = small1.(size 2) in
+  let small13 = small1.(size 3) in
+  let small20 = small2.(size 0) in
+  let small21 = small2.(size 1) in
+  let small22 = small2.(size 2) in
+  let small23 = small2.(size 3) in
 
-  let open FStar.UInt128 in
   let a = mul_wide small10 small20 in
-  let low = uint64_to_uint128 (uint128_to_uint64 a) in
-  let high = a >>^ 64ul in
+  let low = to_u128 (to_u64 a) in
+  let high = a >>. to_shiftval 64 in
   let out0 = low in
   let out1 = high in
 
   let a = mul_wide small10 small21 in
-  let low = uint64_to_uint128 (uint128_to_uint64 a) in
-  let high = a >>^ 64ul in
-  let out1 = out1 +^ low in
+  let low = to_u128 (to_u64 a) in
+  let high = a >>. to_shiftval 64 in
+  let out1 = out1 +. low in
   let out2 = high in
 
   let a = mul_wide small11 small20 in
-  let low = uint64_to_uint128 (uint128_to_uint64 a) in
-  let high = a >>^ 64ul in
-  let out1 = out1 +^ low in
-  let out2 = out2 +^ high in
+  let low = to_u128 (to_u64 a) in
+  let high = a >>. to_shiftval 64 in
+  let out1 = out1 +. low in
+  let out2 = out2 +. high in
 
   let a = mul_wide small10 small22 in
-  let low = uint64_to_uint128 (uint128_to_uint64 a) in
-  let high = a >>^ 64ul in
-  let out2 = out2 +^ low in
+  let low = to_u128 (to_u64 a) in
+  let high = a >>. to_shiftval 64 in
+  let out2 = out2 +. low in
   let out3 = high in
 
   let a = mul_wide small11 small21 in
-  let low = uint64_to_uint128 (uint128_to_uint64 a) in
-  let high = a >>^ 64ul in
-  let out2 = out2 +^ low in
-  let out3 = out3 +^ high in
+  let low = to_u128 (to_u64 a) in
+  let high = a >>. to_shiftval 64 in
+  let out2 = out2 +. low in
+  let out3 = out3 +. high in
 
   let a = mul_wide small12 small20 in
-  let low = uint64_to_uint128 (uint128_to_uint64 a) in
-  let high = a >>^ 64ul in
-  let out2 = out2 +^ low in
-  let out3 = out3 +^ high in
+  let low = to_u128 (to_u64 a) in
+  let high = a >>. to_shiftval 64 in
+  let out2 = out2 +. low in
+  let out3 = out3 +. high in
 
   let a = mul_wide small10 small23 in
-  let low = uint64_to_uint128 (uint128_to_uint64 a) in
-  let high = a >>^ 64ul in
-  let out3 = out3 +^ low in
+  let low = to_u128 (to_u64 a) in
+  let high = a >>. to_shiftval 64 in
+  let out3 = out3 +. low in
   let out4 = high in
 
   let a = mul_wide small11 small22 in
-  let low = uint64_to_uint128 (uint128_to_uint64 a) in
-  let high = a >>^ 64ul in
-  let out3 = out3 +^ low in
-  let out4 = out4 +^ high in
+  let low = to_u128 (to_u64 a) in
+  let high = a >>. to_shiftval 64 in
+  let out3 = out3 +. low in
+  let out4 = out4 +. high in
 
   let a = mul_wide small12 small21 in
-  let low = uint64_to_uint128 (uint128_to_uint64 a) in
-  let high = a >>^ 64ul in
-  let out3 = out3 +^ low in
-  let out4 = out4 +^ high in
+  let low = to_u128 (to_u64 a) in
+  let high = a >>. to_shiftval 64 in
+  let out3 = out3 +. low in
+  let out4 = out4 +. high in
 
   let a = mul_wide small13 small20 in
-  let low = uint64_to_uint128 (uint128_to_uint64 a) in
-  let high = a >>^ 64ul in
-  let out3 = out3 +^ low in
-  let out4 = out4 +^ high in
+  let low = to_u128 (to_u64 a) in
+  let high = a >>. to_shiftval 64 in
+  let out3 = out3 +. low in
+  let out4 = out4 +. high in
 
   let a = mul_wide small11 small23 in
-  let low = uint64_to_uint128 (uint128_to_uint64 a) in
-  let high = a >>^ 64ul in
-  let out4 = out4 +^ low in
+  let low = to_u128 (to_u64 a) in
+  let high = a >>. to_shiftval 64 in
+  let out4 = out4 +. low in
   let out5 = high in
 
   let a = mul_wide small12 small22 in
-  let low = uint64_to_uint128 (uint128_to_uint64 a) in
-  let high = a >>^ 64ul in
-  let out4 = out4 +^ low in
-  let out5 = out5 +^ high in
+  let low = to_u128 (to_u64 a) in
+  let high = a >>. to_shiftval 64 in
+  let out4 = out4 +. low in
+  let out5 = out5 +. high in
 
   let a = mul_wide small13 small21 in
-  let low = uint64_to_uint128 (uint128_to_uint64 a) in
-  let high = a >>^ 64ul in
-  let out4 = out4 +^ low in
-  let out5 = out5 +^ high in
+  let low = to_u128 (to_u64 a) in
+  let high = a >>. to_shiftval 64 in
+  let out4 = out4 +. low in
+  let out5 = out5 +. high in
 
   let a = mul_wide small12 small23 in
-  let low = uint64_to_uint128 (uint128_to_uint64 a) in
-  let high = a >>^ 64ul in
-  let out5 = out5 +^ low in
+  let low = to_u128 (to_u64 a) in
+  let high = a >>. to_shiftval 64 in
+  let out5 = out5 +. low in
   let out6 = high in
 
   let a = mul_wide small13 small22 in
-  let low = uint64_to_uint128 (uint128_to_uint64 a) in
-  let high = a >>^ 64ul in
-  let out5 = out5 +^ low in
-  let out6 = out6 +^ high in
+  let low = to_u128 (to_u64 a) in
+  let high = a >>. to_shiftval 64 in
+  let out5 = out5 +. low in
+  let out6 = out6 +. high in
 
   let a = mul_wide small13 small23 in
-  let low = uint64_to_uint128 (uint128_to_uint64 a) in
-  let high = a >>^ 64ul in
-  let out6 = out6 +^ low in
+  let low = to_u128 (to_u64 a) in
+  let high = a >>. to_shiftval 64 in
+  let out6 = out6 +. low in
   let out7 = high in
 
-  out.(0ul) <- out0;
-  out.(1ul) <- out1;
-  out.(2ul) <- out2;
-  out.(3ul) <- out3;
-  out.(4ul) <- out4;
-  out.(5ul) <- out5;
-  out.(6ul) <- out6;
-  out.(7ul) <- out7
+  out.(size 0) <- out0;
+  out.(size 1) <- out1;
+  out.(size 2) <- out2;
+  out.(size 3) <- out3;
+  out.(size 4) <- out4;
+  out.(size 5) <- out5;
+  out.(size 6) <- out6;
+  out.(size 7) <- out7
 
 val felem_mul:
   out:longfelem -> in1:felem -> in2:felem -> Stack unit
@@ -757,8 +755,8 @@ val felem_mul:
     (ensures (fun h0 _ h1 -> True))
 let felem_mul out in1 in2 =
   push_frame();
-  let small1 = create 0uL 4ul in
-  let small2 = create 0uL 4ul in
+  let small1 = create (size 4) (u64 0) in
+  let small2 = create (size 4) (u64 0) in
   felem_shrink small1 in1;
   felem_shrink small2 in2;
   smallfelem_mul out small1 small2;
@@ -770,7 +768,7 @@ val felem_small_mul:
     (ensures (fun h0 _ h1 -> True))
 let felem_small_mul out small1 in2 =
   push_frame();
-  let small2 = create 0uL 4ul in
+  let small2 = create (size 4) (u64 0) in
   felem_shrink small2 in2;
   smallfelem_mul out small1 small2;
   pop_frame()
@@ -780,43 +778,43 @@ val felem_reduce_:
     (requires (fun h -> True))
     (ensures (fun h0 _ h1 -> True))
 let felem_reduce_ out input =
-  let out0 = out.(0ul) in
-  let out1 = out.(1ul) in
-  let out2 = out.(2ul) in
-  let out3 = out.(3ul) in
-  let input0 = input.(0ul) in
-  let input1 = input.(1ul) in
-  let input2 = input.(2ul) in
-  let input3 = input.(3ul) in
-  let input4 = input.(4ul) in
-  let input5 = input.(5ul) in
-  let input6 = input.(6ul) in
-  let input7 = input.(7ul) in
+  let out0 = out.(size 0) in
+  let out1 = out.(size 1) in
+  let out2 = out.(size 2) in
+  let out3 = out.(size 3) in
+  let input0 = input.(size 0) in
+  let input1 = input.(size 1) in
+  let input2 = input.(size 2) in
+  let input3 = input.(size 3) in
+  let input4 = input.(size 4) in
+  let input5 = input.(size 5) in
+  let input6 = input.(size 6) in
+  let input7 = input.(size 7) in
   let open FStar.UInt128 in
-  let c = input4 +^ (input5 <<^ 32ul) in
-  let out0 = out0 +^ c in
-  let out3 = out3 -^ c in
-  // let c = input5 -^ input7 in
-  let out1 = out1 +^ input5 -^ input7 in
-  let out2 = out2 +^ input7 -^ input5 in
-  // let out1 = out1 +^ c in
-  // let out2 = out2 -^ c in
-  let out1 = out1 -^ (input4 <<^ 32ul) in
-  let out3 = out3 +^ (input4 <<^ 32ul) in
-  let out2 = out2 -^ (input5 <<^ 32ul) in
-  let out0 = out0 -^ input6 in
-  let out0 = out0 -^ (input6 <<^ 32ul) in
-  let out1 = out1 +^ (input6 <<^ 33ul) in
-  let out2 = out2 +^ (input6 <<^ 1ul)  in
-  let out3 = out3 -^ (input6 <<^ 32ul) in
-  let out0 = out0 -^ input7 in
-  let out0 = out0 -^ (input7 <<^ 32ul) in
-  let out2 = out2 +^ (input7 <<^ 33ul) in
-  let out3 = out3 +^ ((input7 <<^ 1ul) +^ input7) in
-  out.(0ul) <- out0;
-  out.(1ul) <- out1;
-  out.(2ul) <- out2;
-  out.(3ul) <- out3
+  let c = input4 +. (input5 <<. to_shiftval 32) in
+  let out0 = out0 +. c in
+  let out3 = out3 -. c in
+  // let c = input5 -. input7 in
+  let out1 = out1 +. input5 -. input7 in
+  let out2 = out2 +. input7 -. input5 in
+  // let out1 = out1 +. c in
+  // let out2 = out2 -. c in
+  let out1 = out1 -. (input4 <<. to_shiftval 32) in
+  let out3 = out3 +. (input4 <<. to_shiftval 32) in
+  let out2 = out2 -. (input5 <<. to_shiftval 32) in
+  let out0 = out0 -. input6 in
+  let out0 = out0 -. (input6 <<. to_shiftval 32) in
+  let out1 = out1 +. (input6 <<. to_shiftval 33) in
+  let out2 = out2 +. (input6 <<. to_shiftval 1)  in
+  let out3 = out3 -. (input6 <<. to_shiftval 32) in
+  let out0 = out0 -. input7 in
+  let out0 = out0 -. (input7 <<. to_shiftval 32) in
+  let out2 = out2 +. (input7 <<. to_shiftval 33) in
+  let out3 = out3 +. ((input7 <<. to_shiftval 1) +. input7) in
+  out.(size 0) <- out0;
+  out.(size 1) <- out1;
+  out.(size 2) <- out2;
+  out.(size 3) <- out3
 
 val felem_reduce:
   out:felem -> input:longfelem -> Stack unit
@@ -826,18 +824,18 @@ let felem_reduce out input =
   let open FStar.UInt128 in
   push_frame();
   let zero100 = zero100() in
-  let zero0 = zero100.(0ul) in
-  let zero1 = zero100.(1ul) in
-  let zero2 = zero100.(2ul) in
-  let zero3 = zero100.(3ul) in
-  let input0 = input.(0ul) in
-  let input1 = input.(1ul) in
-  let input2 = input.(2ul) in
-  let input3 = input.(3ul) in
-  out.(0ul) <- input0 +^ zero0;
-  out.(1ul) <- input1 +^ zero1;
-  out.(2ul) <- input2 +^ zero2;
-  out.(3ul) <- input3 +^ zero3;
+  let zero0 = zero100.(size 0) in
+  let zero1 = zero100.(size 1) in
+  let zero2 = zero100.(size 2) in
+  let zero3 = zero100.(size 3) in
+  let input0 = input.(size 0) in
+  let input1 = input.(size 1) in
+  let input2 = input.(size 2) in
+  let input3 = input.(size 3) in
+  out.(size 0) <- input0 +. zero0;
+  out.(size 1) <- input1 +. zero1;
+  out.(size 2) <- input2 +. zero2;
+  out.(size 3) <- input3 +. zero3;
   felem_reduce_ out input;
   pop_frame()
 
@@ -849,29 +847,29 @@ let felem_reduce_zero105 out input =
   let open FStar.UInt128 in
   push_frame();
   let zero105 = zero105() in
-  let zero0 = zero105.(0ul) in
-  let zero1 = zero105.(1ul) in
-  let zero2 = zero105.(2ul) in
-  let zero3 = zero105.(3ul) in
-  let input0 = input.(0ul) in
-  let input1 = input.(1ul) in
-  let input2 = input.(2ul) in
-  let input3 = input.(3ul) in
-  out.(0ul) <- input0 +^ zero0;
-  out.(1ul) <- input1 +^ zero1;
-  out.(2ul) <- input2 +^ zero2;
-  out.(3ul) <- input3 +^ zero3;
+  let zero0 = zero105.(size 0) in
+  let zero1 = zero105.(size 1) in
+  let zero2 = zero105.(size 2) in
+  let zero3 = zero105.(size 3) in
+  let input0 = input.(size 0) in
+  let input1 = input.(size 1) in
+  let input2 = input.(size 2) in
+  let input3 = input.(size 3) in
+  out.(size 0) <- input0 +. zero0;
+  out.(size 1) <- input1 +. zero1;
+  out.(size 2) <- input2 +. zero2;
+  out.(size 3) <- input3 +. zero3;
   felem_reduce_ out input;
   pop_frame()
 
 val subtract_u64:
-  result:u64 -> v:u64 -> Tot (tuple2 u64 u64)
+  result:uint64 -> v:uint64 -> Tot (tuple2 uint64 uint64)
 let subtract_u64 result v' =
-  let r = UInt128.uint64_to_uint128 result in
-  let r = FStar.UInt128.(r -%^ uint64_to_uint128 v') in  
-  let open FStar.UInt64 in
-  let carry = FStar.UInt128.(uint128_to_uint64 (r >>^ 64ul)) &^ 1uL in
-  let result = UInt128.uint128_to_uint64 r in
+  let r = to_u128 result in
+  let r = r -. to_u128 v' in
+  (* WAS let r = (r -%^ to_u128 v') in *)
+  let carry = (to_u64 (r >>. to_shiftval 64)) &. (u64 1) in
+  let result = to_u64 r in
   result, carry
 
 val felem_contract:
@@ -880,85 +878,84 @@ val felem_contract:
     (ensures (fun h0 _ h1 -> True))
 let felem_contract out input =
   push_frame();
-  let all_equal_so_far = 0uL in
-  let result = 0uL in
+  let all_equal_so_far = u64 0 in
+  let result = u64 0 in
   felem_shrink out input;
-  let all_equal_so_far = FStar.UInt64.(all_equal_so_far -%^ 1uL) in
+  let all_equal_so_far = all_equal_so_far -. (u64 1) in
+  (* WAS let all_equal_so_far = FStar.UInt64.(all_equal_so_far -%^ 1uL) in *)
 
-  let open FStar.UInt128 in
   let kPrime = kPrime() in
-  let kPrime0 = kPrime.(0ul) in
-  let kPrime1 = kPrime.(1ul) in
-  let kPrime2 = kPrime.(2ul) in
-  let kPrime3 = kPrime.(3ul) in
-  let out0 = out.(0ul) in
-  let out1 = out.(1ul) in
-  let out2 = out.(2ul) in
-  let out3 = out.(3ul) in
-  let a = uint64_to_uint128 kPrime0 -^ uint64_to_uint128 out0 in
-  let result = FStar.UInt64.(result |^ (all_equal_so_far &^ FStar.UInt128.(uint128_to_uint64 (a >>^ 64ul)))) in
+  let kPrime0 = kPrime.(size 0) in
+  let kPrime1 = kPrime.(size 1) in
+  let kPrime2 = kPrime.(size 2) in
+  let kPrime3 = kPrime.(size 3) in
+  let out0 = out.(size 0) in
+  let out1 = out.(size 1) in
+  let out2 = out.(size 2) in
+  let out3 = out.(size 3) in
+  let a = to_u128 kPrime0 -. to_u128 out0 in
+  let result = (result |. (all_equal_so_far &. (to_u64 (a >>. to_shiftval 64)))) in
 
-  let open FStar.UInt64 in
-  let equal = kPrime3 ^^ out3 in
-  let equal = equal -^ 1uL in
-  let equal = equal &^ (equal <<^ 32ul) in
-  let equal = equal &^ (equal <<^ 16ul) in
-  let equal = equal &^ (equal <<^ 8ul) in
-  let equal = equal &^ (equal <<^ 4ul) in
-  let equal = equal &^ (equal <<^ 2ul) in
-  let equal = equal &^ (equal <<^ 1ul) in
-  let equal = gte_mask equal 0x1000000000000000uL in
-  let all_equal_so_far = all_equal_so_far &^ equal in
+  let equal = kPrime3 ^. out3 in
+  let equal = equal -. (u64 1) in
+  let equal = equal &. (equal <<. to_shiftval 32) in
+  let equal = equal &. (equal <<. to_shiftval 16) in
+  let equal = equal &. (equal <<. to_shiftval 8) in
+  let equal = equal &. (equal <<. to_shiftval 4) in
+  let equal = equal &. (equal <<. to_shiftval 2) in
+  let equal = equal &. (equal <<. to_shiftval 1) in
+  let equal = gte_mask equal (u64 0x1000000000000000) in
+  let all_equal_so_far = all_equal_so_far &. equal in
 
 
-  let equal = kPrime2 ^^ out2 in
-  let equal = equal -^ 1uL in
-  let equal = equal &^ (equal <<^ 32ul) in
-  let equal = equal &^ (equal <<^ 16ul) in
-  let equal = equal &^ (equal <<^ 8ul) in
-  let equal = equal &^ (equal <<^ 4ul) in
-  let equal = equal &^ (equal <<^ 2ul) in
-  let equal = equal &^ (equal <<^ 1ul) in
-  let equal = gte_mask equal 0x1000000000000000uL in
-  let all_equal_so_far = all_equal_so_far &^ equal in
+  let equal = kPrime2 ^. out2 in
+  let equal = equal -. (u64 1) in
+  let equal = equal &. (equal <<. to_shiftval 32) in
+  let equal = equal &. (equal <<. to_shiftval 16) in
+  let equal = equal &. (equal <<. to_shiftval 8) in
+  let equal = equal &. (equal <<. to_shiftval 4) in
+  let equal = equal &. (equal <<. to_shiftval 2) in
+  let equal = equal &. (equal <<. to_shiftval 1) in
+  let equal = gte_mask equal (u64 0x1000000000000000) in
+  let all_equal_so_far = all_equal_so_far &. equal in
 
-  let equal = kPrime1 ^^ out1 in
-  let equal = equal -^ 1uL in
-  let equal = equal &^ (equal <<^ 32ul) in
-  let equal = equal &^ (equal <<^ 16ul) in
-  let equal = equal &^ (equal <<^ 8ul) in
-  let equal = equal &^ (equal <<^ 4ul) in
-  let equal = equal &^ (equal <<^ 2ul) in
-  let equal = equal &^ (equal <<^ 1ul) in
-  let equal = gte_mask equal 0x1000000000000000uL in
-  let all_equal_so_far = all_equal_so_far &^ equal in
+  let equal = kPrime1 ^. out1 in
+  let equal = equal -. (u64 1) in
+  let equal = equal &. (equal <<. to_shiftval 32) in
+  let equal = equal &. (equal <<. to_shiftval 16) in
+  let equal = equal &. (equal <<. to_shiftval 8) in
+  let equal = equal &. (equal <<. to_shiftval 4) in
+  let equal = equal &. (equal <<. to_shiftval 2) in
+  let equal = equal &. (equal <<. to_shiftval 1) in
+  let equal = gte_mask equal (u64 0x1000000000000000) in
+  let all_equal_so_far = all_equal_so_far &. equal in
 
-  let equal = kPrime0 ^^ out0 in
-  let equal = equal -^ 1uL in
-  let equal = equal &^ (equal <<^ 32ul) in
-  let equal = equal &^ (equal <<^ 16ul) in
-  let equal = equal &^ (equal <<^ 8ul) in
-  let equal = equal &^ (equal <<^ 4ul) in
-  let equal = equal &^ (equal <<^ 2ul) in
-  let equal = equal &^ (equal <<^ 1ul) in
-  let equal = gte_mask equal 0x1000000000000000uL in
-  let all_equal_so_far = all_equal_so_far &^ equal in
+  let equal = kPrime0 ^. out0 in
+  let equal = equal -. (u64 1) in
+  let equal = equal &. (equal <<. to_shiftval 32) in
+  let equal = equal &. (equal <<. to_shiftval 16) in
+  let equal = equal &. (equal <<. to_shiftval 8) in
+  let equal = equal &. (equal <<. to_shiftval 4) in
+  let equal = equal &. (equal <<. to_shiftval 2) in
+  let equal = equal &. (equal <<. to_shiftval 1) in
+  let equal = gte_mask equal (u64 0x1000000000000000) in
+  let all_equal_so_far = all_equal_so_far &. equal in
 
-  let result = result |^ all_equal_so_far in
+  let result = result |. all_equal_so_far in
 
-  let out0, carry = subtract_u64 out0 (result &^ kPrime0) in
+  let out0, carry = subtract_u64 out0 (result &. kPrime0) in
   let out1, carry = subtract_u64 out1 carry in
   let out2, carry = subtract_u64 out2 carry in
   let out3, carry = subtract_u64 out3 carry in
 
-  let out1, carry = subtract_u64 out1 (result &^ kPrime1) in
+  let out1, carry = subtract_u64 out1 (result &. kPrime1) in
   let out2, carry = subtract_u64 out2 carry in
   let out3, carry = subtract_u64 out3 carry in
 
-  let out2, carry = subtract_u64 out2 (result &^ kPrime2) in
+  let out2, carry = subtract_u64 out2 (result &. kPrime2) in
   let out3, carry = subtract_u64 out3 carry in
 
-  let out3, carry = subtract_u64 out3 (result &^ kPrime3) in
+  let out3, carry = subtract_u64 out3 (result &. kPrime3) in
   pop_frame()
 
 val smallfelem_mul_contract:
@@ -967,8 +964,8 @@ val smallfelem_mul_contract:
     (ensures (fun h0 _ h1 -> True))
 let smallfelem_mul_contract out in1 in2 =
   push_frame();
-  let longtmp = create (UInt128.uint64_to_uint128 0uL) 8ul in
-  let tmp     = create (UInt128.uint64_to_uint128 0uL) 4ul in
+  let longtmp = create (size 8) (u128 0) in
+  let tmp     = create (size 4) (u128 0) in
   smallfelem_mul longtmp in1 in2;
   felem_reduce tmp longtmp;
   felem_contract out tmp;
@@ -981,31 +978,30 @@ val smallfelem_is_zero:
 let smallfelem_is_zero small =
   push_frame();
   let kPrime = kPrime() in
-  let kPrime0 = kPrime.(0ul) in
-  let kPrime1 = kPrime.(1ul) in
-  let kPrime2 = kPrime.(2ul) in
-  let kPrime3 = kPrime.(3ul) in
-  let small0 = small.(0ul) in
-  let small1 = small.(1ul) in
-  let small2 = small.(2ul) in
-  let small3 = small.(3ul) in
-  let open FStar.UInt64 in
-  let is_zero = FStar.UInt64.(small0 |^ small1 |^ small2 |^ small3) in
-  let is_zero = eq_mask is_zero 0uL in
-  let is_p = (small0 ^^ kPrime0) |^ (small1 ^^ kPrime1) |^ (small2 ^^ kPrime2) |^ (small3 ^^ kPrime3) in
-  let is_p = eq_mask is_p 0uL in
-  let is_zero = is_zero |^ is_p in
-  let result = FStar.UInt128.(uint64_to_uint128 is_zero |^ (uint64_to_uint128 is_zero <<^ 64ul)) in
+  let kPrime0 = kPrime.(size 0) in
+  let kPrime1 = kPrime.(size 1) in
+  let kPrime2 = kPrime.(size 2) in
+  let kPrime3 = kPrime.(size 3) in
+  let small0 = small.(size 0) in
+  let small1 = small.(size 1) in
+  let small2 = small.(size 2) in
+  let small3 = small.(size 3) in
+  let is_zero = (small0 |. small1 |. small2 |. small3) in
+  let is_zero = eq_mask is_zero (u64 0) in
+  let is_p = (small0 ^. kPrime0) |. (small1 ^. kPrime1) |. (small2 ^. kPrime2) |. (small3 ^. kPrime3) in
+  let is_p = eq_mask is_p (u64 0) in
+  let is_zero = is_zero |. is_p in
+  let result = (to_u128 is_zero |. (to_u128 is_zero <<. to_shiftval 64)) in
   pop_frame();
   result
 
 val smallfelem_is_zero_int:
-  small:smallfelem -> Stack FStar.UInt32.t
+  small:smallfelem -> Stack uint32
     (requires (fun h -> True))
     (ensures (fun h0 _ h1 -> True))
 let smallfelem_is_zero_int small =
   let w = smallfelem_is_zero small in
-  FStar.UInt128.(uint64_to_uint32 (uint128_to_uint64 (w &^ uint64_to_uint128 1uL)))
+  to_u32 (to_u64 (w &. (u128 1)))
 
 val felem_inv:
   out:felem -> input:felem -> Stack unit
@@ -1013,16 +1009,16 @@ val felem_inv:
     (ensures (fun h0 _ h1 -> True))
 let felem_inv out input =
   push_frame();
-  let z = FStar.UInt128.uint64_to_uint128 0uL in
-  let ftmp = create z 4ul in
-  let ftmp2 = create z 4ul in
-  let e2 = create z 4ul in
-  let e4 = create z 4ul in
-  let e8 = create z 4ul in
-  let e16 = create z 4ul in
-  let e32 = create z 4ul in
-  let e64 = create z 4ul in
-  let tmp = create z 8ul in
+  let z = u128 0 in
+  let ftmp = create (size 4) z in
+  let ftmp2 = create (size 4) z in
+  let e2 = create (size 4) z in
+  let e4 = create (size 4) z in
+  let e8 = create (size 4) z in
+  let e16 = create (size 4) z in
+  let e32 = create (size 4) z in
+  let e64 = create (size 4) z in
+  let tmp = create (size 4) z in
   felem_square tmp input;
   felem_reduce ftmp tmp;
   felem_mul tmp input ftmp;
@@ -1104,7 +1100,7 @@ val smallfelem_inv_contract:
     (ensures (fun h0 _ h1 -> True))
 let smallfelem_inv_contract out input =
   push_frame();
-  let tmp = create (UInt128.uint64_to_uint128 0uL) 4ul in
+  let tmp = create (UInt128.to_u128 0uL) 4ul in
   smallfelem_expand tmp input;
   felem_inv tmp tmp;
   felem_contract out tmp;
@@ -1123,14 +1119,14 @@ val point_double:
     (ensures (fun h0 _ h1 -> True))
 let point_double x_out y_out z_out x_in y_in z_in =
   push_frame();
-  let tmp = create (UInt128.uint64_to_uint128 0uL) 8ul in
-  let tmp2 = create (UInt128.uint64_to_uint128 0uL) 8ul in
-  let delta = create (UInt128.uint64_to_uint128 0uL) 4ul in
-  let gamma = create (UInt128.uint64_to_uint128 0uL) 4ul in
-  let beta = create (UInt128.uint64_to_uint128 0uL) 4ul in
-  let alpha = create (UInt128.uint64_to_uint128 0uL) 4ul in
-  let ftmp = create (UInt128.uint64_to_uint128 0uL) 4ul in
-  let ftmp2 = create (UInt128.uint64_to_uint128 0uL) 4ul in
+  let tmp = create (UInt128.to_u128 0uL) 8ul in
+  let tmp2 = create (UInt128.to_u128 0) 8ul in
+  let delta = create (UInt128.to_u128 0) 4ul in
+  let gamma = create (UInt128.to_u128 0) 4ul in
+  let beta = create (UInt128.to_u128 0) 4ul in
+  let alpha = create (UInt128.to_u128 0) 4ul in
+  let ftmp = create (UInt128.to_u128 0) 4ul in
+  let ftmp2 = create (UInt128.to_u128 0) 4ul in
   let small1 = create 0uL 4ul in
   let small2 = create 0uL 4ul in
 
@@ -1179,7 +1175,7 @@ let point_double x_out y_out z_out x_in y_in z_in =
   longfelem_diff tmp tmp2;
   felem_reduce_zero105 y_out tmp;
   pop_frame()
-  
+
 
 val point_double_small:
   x_out:smallfelem -> y_out:smallfelem -> z_out:smallfelem ->
@@ -1213,8 +1209,8 @@ let copy_conditional out input mask =
     (ensures (fun h0 _ h1 -> True))
     = let inputi = input.(i) in
       let outi = out.(i) in
-      let tmp = mask &^ (inputi ^^ outi) in
-      // let tmp = mask &^ input.(FStar.UInt32.(nlimbs' -^ 1ul -^ i)) in
+      let tmp = mask &. (inputi ^^ outi) in
+      // let tmp = mask &. input.(FStar.UInt32.(nlimbs' -. 1ul -. i)) in
       out.(i) <- outi ^^ tmp in
   for 0ul nlimbs' inv f
 
@@ -1224,14 +1220,14 @@ val copy_small_conditional:
     (ensures (fun h0 _ h1 -> True))
 let copy_small_conditional out input mask =
   let open FStar.UInt128 in
-  let mask64 = uint128_to_uint64 mask in
+  let mask64 = to_u64 mask in
   let inv (h1:mem) (i:nat) = True in
   let f (i:UInt32.t) : Stack unit
     (requires (fun h -> True))
     (ensures (fun h0 _ h1 -> True))
     = let inputi = input.(i) in
       let outi = out.(i) in
-      let tmp = (uint64_to_uint128 FStar.UInt64.(inputi &^ mask64) |^ (outi &^ lognot mask)) in
+      let tmp = (to_u128 FStar.UInt64.(inputi &. mask64) |^ (outi &. lognot mask)) in
       out.(i) <- tmp in
   for 0ul nlimbs' inv f
 
@@ -1327,7 +1323,7 @@ let point_add x3 y3 z3 x1 y1 z1 mixed x2 y2 z2 =
   felem_shrink small1 ftmp5;
   let y_equal = smallfelem_is_zero small1 in
 
-  let zero = UInt128.uint64_to_uint128 0uL in
+  let zero = UInt128.to_u128 0uL in
   if  ((x_equal <> zero) && (y_equal <> zero) && not(z1_is_zero <> zero) && not(z2_is_zero <> zero)) then
       begin
         point_double x3 y3 z3 x1 y1 z1
@@ -1423,13 +1419,13 @@ let ith_bit k i =
   let open FStar.UInt32 in
   let q = i >>^ 3ul in
   assert(v q = v i / 8);
-  let r = i &^ 7ul in
+  let r = i &. 7ul in
   UInt.logand_mask (v i) 3;
   assert(v r = v i % 8);
   Math.Lemmas.lemma_div_lt (v i) 8 3;
   let kq = k.(q) in
   let kq' = Hacl.UInt8.(kq >>^ r) in
-  let z = Hacl.UInt8.(kq' &^ Hacl.Cast.uint8_to_sint8 1uy) in
+  let z = Hacl.UInt8.(kq' &. Hacl.Cast.uint8_to_sint8 1uy) in
   UInt.logand_mask (Hacl.UInt8.v kq') 1;
   assert(Hacl.UInt8.v z = (Hacl.UInt8.v kq / pow2 (v r)) % 2);
   z
@@ -1437,7 +1433,7 @@ let ith_bit k i =
 private
 inline_for_extraction let mk_mask (iswap:UInt128.t{UInt128.v iswap = 0 \/ UInt128.v iswap = 1}) :
   Tot (z:UInt128.t{if UInt128.v iswap = 1 then UInt128.v z = pow2 64 - 1 else UInt128.v z = 0})
-  = let swap = FStar.UInt128.(uint64_to_uint128 0uL -%^ iswap) in
+  = let swap = FStar.UInt128.(to_u128 0uL -%^ iswap) in
     assert_norm((0 - 1) % pow2 64 = pow2 64 - 1);
     assert_norm((0 - 0) % pow2 64 = 0);
     swap
@@ -1486,7 +1482,7 @@ let swap_cond_inplace p q iswap =
     = let open FStar.UInt128 in
       let pi = p.(i) in
       let qi = q.(i) in
-      let x  = mask &^ (pi ^^ qi) in
+      let x  = mask &. (pi ^^ qi) in
       let pi' = pi ^^ x in
       let qi' = qi ^^ x in
       p.(i) <- pi';
@@ -1526,10 +1522,10 @@ let loop_step pp ppq p pq k i =
   // let x1 = x.(1ul) in
   // let x2 = x.(2ul) in
   // let x3 = x.(3ul) in
-  // ppq.(0ul) <- UInt128.uint64_to_uint128 x0;
-  // ppq.(1ul) <- UInt128.uint64_to_uint128 x1;
-  // ppq.(2ul) <- UInt128.uint64_to_uint128 x2;
-  // ppq.(3ul) <- UInt128.uint64_to_uint128 x3;
+  // ppq.(0ul) <- UInt128.to_u128 x0;
+  // ppq.(1ul) <- UInt128.to_u128 x1;
+  // ppq.(2ul) <- UInt128.to_u128 x2;
+  // ppq.(3ul) <- UInt128.to_u128 x3;
   swap_cond_inplace pp ppq ith_bit;
   pop_frame()
 
@@ -1551,8 +1547,8 @@ let point_mul_ pp ppq p pq k =
     (requires (fun h -> inv h (UInt32.v i)))
     (ensures (fun h_1 _ h_2 -> FStar.UInt32.(inv h_2 (v i + 1))))
   =
-    loop_step pp ppq p pq k FStar.UInt32.(256ul -^ (2ul *^ i) -^ 1ul);
-    loop_step p pq pp ppq k FStar.UInt32.(256ul -^ (2ul *^ i) -^ 2ul)
+    loop_step pp ppq p pq k FStar.UInt32.(256ul -. (2ul *^ i) -. 1ul);
+    loop_step p pq pp ppq k FStar.UInt32.(256ul -. (2ul *^ i) -. 2ul)
   in
   C.Loops.for 0ul 128ul inv f'
 
@@ -1569,7 +1565,7 @@ val p256:
 let p256 outx outy inx iny key =
   push_frame();
   // Initial point
-  let q = create (UInt128.uint64_to_uint128 0uL) 12ul in
+  let q = create (UInt128.to_u128 0uL) 12ul in
   let qx = get_x q in
   let qy = get_y q in
   let qz = get_z q in
@@ -1581,49 +1577,49 @@ let p256 outx outy inx iny key =
   let qy2 = load64_be (Buffer.sub iny 8ul 8ul) in
   let qy1 = load64_be (Buffer.sub iny 16ul 8ul) in
   let qy0 = load64_be (Buffer.sub iny 24ul 8ul) in
-  qx.(0ul) <- UInt128.uint64_to_uint128 qx0;
-  qx.(1ul) <- UInt128.uint64_to_uint128 qx1;
-  qx.(2ul) <- UInt128.uint64_to_uint128 qx2;
-  qx.(3ul) <- UInt128.uint64_to_uint128 qx3;
-  qy.(0ul) <- UInt128.uint64_to_uint128 qy0;
-  qy.(1ul) <- UInt128.uint64_to_uint128 qy1;
-  qy.(2ul) <- UInt128.uint64_to_uint128 qy2;
-  qy.(3ul) <- UInt128.uint64_to_uint128 qy3;
-  qz.(0ul) <- UInt128.uint64_to_uint128 1uL;
+  qx.(0ul) <- UInt128.to_u128 qx0;
+  qx.(1ul) <- UInt128.to_u128 qx1;
+  qx.(2ul) <- UInt128.to_u128 qx2;
+  qx.(3ul) <- UInt128.to_u128 qx3;
+  qy.(0ul) <- UInt128.to_u128 qy0;
+  qy.(1ul) <- UInt128.to_u128 qy1;
+  qy.(2ul) <- UInt128.to_u128 qy2;
+  qy.(3ul) <- UInt128.to_u128 qy3;
+  qz.(0ul) <- UInt128.to_u128 1uL;
   // Create point at infinity
-  let p = create (UInt128.uint64_to_uint128 0uL) 12ul in
+  let p = create (UInt128.to_u128 0uL) 12ul in
   let px = get_x p in
   let py = get_y p in
-  px.(0ul) <- UInt128.uint64_to_uint128 1uL;
-  py.(0ul) <- UInt128.uint64_to_uint128 1uL;
-  let pp = create (UInt128.uint64_to_uint128 0uL) 12ul in
-  let ppq = create (UInt128.uint64_to_uint128 0uL) 12ul in
+  px.(0ul) <- UInt128.to_u128 1uL;
+  py.(0ul) <- UInt128.to_u128 1uL;
+  let pp = create (UInt128.to_u128 0uL) 12ul in
+  let ppq = create (UInt128.to_u128 0uL) 12ul in
   point_mul_ pp ppq p q key;
-  
+
   let x = create 0uL 4ul in
   let y = create 0uL 4ul in
-  let tmp = create (UInt128.uint64_to_uint128 0uL) 8ul in
-  let z2 = create (UInt128.uint64_to_uint128 0uL) 4ul in
-  let z3 = create (UInt128.uint64_to_uint128 0uL) 4ul in
-  let z2_inv = create (UInt128.uint64_to_uint128 0uL) 4ul in
-  let z3_inv = create (UInt128.uint64_to_uint128 0uL) 4ul in
-  let big_x = create (UInt128.uint64_to_uint128 0uL) 4ul in
-  let big_y = create (UInt128.uint64_to_uint128 0uL) 4ul in
-  
+  let tmp = create (UInt128.to_u128 0uL) 8ul in
+  let z2 = create (UInt128.to_u128 0uL) 4ul in
+  let z3 = create (UInt128.to_u128 0uL) 4ul in
+  let z2_inv = create (UInt128.to_u128 0uL) 4ul in
+  let z3_inv = create (UInt128.to_u128 0uL) 4ul in
+  let big_x = create (UInt128.to_u128 0uL) 4ul in
+  let big_y = create (UInt128.to_u128 0uL) 4ul in
+
   felem_square tmp (get_z p);
   felem_reduce z2 tmp;
   felem_inv z2_inv z2;
   felem_mul tmp (get_x p) z2_inv;
   felem_reduce big_x tmp;
   felem_contract x big_x;
-  
+
   felem_mul tmp z2 (get_z p);
   felem_reduce z3 tmp;
   felem_inv z3_inv z3;
   felem_mul tmp (get_y p) z3_inv;
   felem_reduce big_y tmp;
   felem_contract y big_y;
-  
+
   let x0 = x.(0ul) in
   let x1 = x.(1ul) in
   let x2 = x.(2ul) in
